Px86 atop: finish atop
Signed-off-by: Kyeongmin Cho <kyeongmin.cho@kaist.ac.kr>

src/axiomatic/TsoSimLocal.v
@@ -381,15 +381,51 @@ Proof.
   - inv H1. ss. subst. eapply FWDN. econs; eauto. econs; eauto with tso.
 Qed.
 
+Definition sim_local_vpn ex :=
+  (⦗ex.(Execution.label_is) Label.is_kinda_read⦘ ⨾
+   Execution.po) ∪
+
+  (⦗ex.(Execution.label_is) Label.is_access⦘ ⨾
+   Execution.po ⨾
+   (⦗ex.(Execution.label_is) (Label.is_barrier_c Barrier.is_mfence)⦘ ∪
+    ⦗ex.(Execution.label_is) (Label.is_barrier_c Barrier.is_sfence)⦘) ⨾
+   Execution.po).
+
+Lemma sim_local_vpn_step ex:
+  sim_local_vpn ex =
+  (sim_local_vpn ex ∪
+   ((⦗ex.(Execution.label_is) Label.is_kinda_read⦘) ∪
+
+   (⦗ex.(Execution.label_is) Label.is_access⦘ ⨾
+     Execution.po ⨾
+     (⦗ex.(Execution.label_is) (Label.is_barrier_c Barrier.is_mfence)⦘ ∪
+      ⦗ex.(Execution.label_is) (Label.is_barrier_c Barrier.is_sfence)⦘)))) ⨾
+  Execution.po_adj.
+Proof.
+  unfold sim_local_vpn. rewrite ? (union_seq' Execution.po_adj), ? seq_assoc, ? union_assoc.
+  rewrite Execution.po_po_adj at 1 3.
+  rewrite (clos_refl_union Execution.po), union_seq, eq_seq.
+  rewrite ? (seq_union' (Execution.po ⨾ Execution.po_adj) Execution.po_adj), ? seq_assoc, ? union_assoc.
+  funext. i. funext. i. propext. econs; i.
+  - repeat match goal with
+           | [H: (_ ∪ _) _ _ |- _] => inv H
+           end;
+      eauto 10 using union_l, union_r.
+  - repeat match goal with
+           | [H: (_ ∪ _) _ _ |- _] => inv H
+           end;
+      eauto 10 using union_l, union_r.
+Qed.
+
 Definition sim_local_lper ex loc :=
-  ((sim_local_coh ex loc ∪ sim_local_vrn ex) ⨾
+  ((sim_local_coh ex loc ∪ sim_local_vpn ex) ⨾
    ⦗ex.(Execution.label_is) (Label.is_flushopting loc)⦘ ⨾
    Execution.po).
 
 Lemma sim_local_lper_step ex loc:
   sim_local_lper ex loc =
   (sim_local_lper ex loc ∪
-   ((sim_local_coh ex loc ∪ sim_local_vrn ex) ⨾
+   ((sim_local_coh ex loc ∪ sim_local_vpn ex) ⨾
     ⦗ex.(Execution.label_is) (Label.is_flushopting loc)⦘)) ⨾
   Execution.po_adj.
 Proof.
@@ -405,31 +441,44 @@ Proof.
 Qed.
 
 Definition sim_local_per ex loc :=
-  ((sim_local_coh ex loc ∪ sim_local_vrn ex) ⨾
-   (⦗ex.(Execution.label_is) (Label.is_flushing loc)⦘ ∪
-    (⦗ex.(Execution.label_is) (Label.is_flushopting loc)⦘ ⨾
-     Execution.po ⨾
-     ⦗ex.(Execution.label_is) (Label.is_persist_barrier)⦘)) ⨾
+  (sim_local_vwn ex ⨾
+   ⦗ex.(Execution.label_is) (Label.is_flushing loc)⦘ ⨾
+   Execution.po) ∪
+
+  ((sim_local_coh ex loc ∪ sim_local_vpn ex) ⨾
+   ⦗ex.(Execution.label_is) (Label.is_flushopting loc)⦘ ⨾
+   Execution.po ⨾
+   ⦗ex.(Execution.label_is) (Label.is_persist_barrier)⦘ ⨾
    Execution.po).
 
 Lemma sim_local_per_step ex loc:
   sim_local_per ex loc =
   (sim_local_per ex loc ∪
-   (sim_local_coh ex loc ∪ sim_local_vrn ex) ⨾
-   (⦗ex.(Execution.label_is) (Label.is_flushing loc)⦘ ∪
-    (⦗ex.(Execution.label_is) (Label.is_flushopting loc)⦘ ⨾
-     Execution.po ⨾
-     ⦗ex.(Execution.label_is) (Label.is_persist_barrier)⦘))) ⨾
+   ((sim_local_vwn ex ⨾
+    ⦗ex.(Execution.label_is) (Label.is_flushing loc)⦘) ∪
+
+    ((sim_local_coh ex loc ∪ sim_local_vpn ex) ⨾
+    ⦗ex.(Execution.label_is) (Label.is_flushopting loc)⦘ ⨾
+    Execution.po ⨾
+    ⦗ex.(Execution.label_is) (Label.is_persist_barrier)⦘))) ⨾
   Execution.po_adj.
 Proof.
   unfold sim_local_per.
   rewrite ? (union_seq' Execution.po_adj), ? seq_assoc, ? union_assoc.
-  rewrite Execution.po_po_adj at 2.
+  rewrite Execution.po_po_adj at 1 3.
   rewrite (clos_refl_union Execution.po).
   replace ((Execution.po ∪ eq) ⨾ Execution.po_adj)
     with (Execution.po ⨾ Execution.po_adj ∪ eq ⨾ Execution.po_adj); cycle 1.
   { rewrite union_seq. ss. }
   rewrite eq_seq.
   rewrite ? (seq_union' (Execution.po ⨾ Execution.po_adj) Execution.po_adj), ? seq_assoc, ? union_assoc.
-  refl.
+  funext. i. funext. i. propext. econs; i.
+  - repeat match goal with
+           | [H: (_ ∪ _) _ _ |- _] => inv H
+           end;
+      eauto 10 using union_l, union_r.
+  - repeat match goal with
+           | [H: (_ ∪ _) _ _ |- _] => inv H
+           end;
+      eauto 10 using union_l, union_r.
 Qed.
